

## CHAPTER 7 – SYSTEM OF LINEAR EQUATIONS

### Part 1. System of Linear equations

#### Exercise 1.

In Problems 33–46, solve each system of equations using the method of substitution. If the system has no solution, say that it is inconsistent

$$33. \begin{cases} 2x + 3y = 6 \\ x - y = \frac{1}{2} \end{cases}$$

$$34. \begin{cases} \frac{1}{2}x + y = -2 \\ x - 2y = 8 \end{cases}$$

$$35. \begin{cases} \frac{1}{2}x + \frac{1}{3}y = 3 \\ \frac{1}{4}x - \frac{2}{3}y = -1 \end{cases}$$

$$36. \begin{cases} \frac{1}{3}x - \frac{3}{2}y = -5 \\ \frac{3}{4}x + \frac{1}{3}y = 11 \end{cases}$$

$$37. \begin{cases} 3x - 5y = 3 \\ 15x + 5y = 21 \end{cases}$$

$$38. \begin{cases} 2x - y = -1 \\ x + \frac{1}{2}y = \frac{3}{2} \end{cases}$$

$$39. \begin{cases} \frac{1}{x} + \frac{1}{y} = 8 \\ \frac{3}{x} - \frac{5}{y} = 0 \end{cases}$$

$$40. \begin{cases} \frac{4}{x} - \frac{3}{y} = 0 \\ \frac{6}{x} + \frac{3}{2y} = 2 \end{cases}$$

$$41. \begin{cases} x - y = 6 \\ 2x - 3z = 16 \\ 2y + z = 4 \end{cases}$$

$$42. \begin{cases} 2x + y = -4 \\ -2y + 4z = 0 \\ 3x - 2z = -11 \end{cases}$$

$$43. \begin{cases} x - 2y + 3z = 7 \\ 2x + y + z = 4 \\ -3x + 2y - 2z = -10 \end{cases}$$

$$44. \begin{cases} 2x + y - 3z = 0 \\ -2x + 2y + z = -7 \\ 3x - 4y - 3z = 7 \end{cases}$$

$$45. \begin{cases} x - y - z = 1 \\ 2x + 3y + z = 2 \\ 3x + 2y = 0 \end{cases}$$

$$46. \begin{cases} 2x - 3y - z = 0 \\ -x + 2y + z = 5 \\ 3x - 4y - z = 1 \end{cases}$$

#### Exercise 2.

- 1) The perimeter of a rectangular floor is 90 feet. Find the dimensions of the floor if the length is twice the width?
- 2) Financial Planning A recently retired couple needs \$12,000 per year to supplement their Social Security. They have \$150,000 to invest to obtain this income. They have decided on two investment options: AA bonds yielding 10% per annum and a Bank Certificate yielding 5%
  - (a) How much should be invested in each to realize exactly \$12,000?
  - (b) If, after 2 years, the couple requires \$14,000 per year in income, how should they reallocate their investment to achieve the new amount?
- 3) Find real numbers  $a, b$  and  $c$  so that the graph of the function  $y = ax^2 + bx + c$  contains the points  $(-1, 4)$ ,  $(2, 3)$  and  $(0, 1)$ .

#### Exercise 3.

In Problems 5–16, write the augmented matrix of the given system of equations.

$$5. \begin{cases} x - 5y = 5 \\ 4x + 3y = 6 \end{cases}$$

$$6. \begin{cases} 3x + 4y = 7 \\ 4x - 2y = 5 \end{cases}$$

$$7. \begin{cases} 2x + 3y - 6 = 0 \\ 4x - 6y + 2 = 0 \end{cases}$$

$$8. \begin{cases} 9x - y = 0 \\ 3x - y - 4 = 0 \end{cases}$$

$$9. \begin{cases} 0.01x - 0.03y = 0.06 \\ 0.13x + 0.10y = 0.20 \end{cases}$$

$$10. \begin{cases} \frac{4}{3}x - \frac{3}{2}y = \frac{3}{4} \\ -\frac{1}{4}x + \frac{1}{3}y = \frac{2}{3} \end{cases}$$

$$11. \begin{cases} x - y + z = 10 \\ 3x + 3y = 5 \\ x + y + 2z = 2 \end{cases}$$

$$12. \begin{cases} 5x - y - z = 0 \\ x + y = 5 \\ 2x - 3z = 2 \end{cases}$$

$$13. \begin{cases} x + y - z = 2 \\ 3x - 2y = 2 \\ 5x + 3y - z = 1 \end{cases}$$

$$14. \begin{cases} 2x + 3y - 4z = 0 \\ x - 5z + 2 = 0 \\ x + 2y - 3z = -2 \end{cases}$$

$$15. \begin{cases} x - y - z = 10 \\ 2x + y + 2z = -1 \\ -3x + 4y = 5 \\ 4x - 5y + z = 0 \end{cases}$$

$$16. \begin{cases} x - y + 2z - w = 5 \\ x + 3y - 4z + 2w = 2 \\ 3x - y - 5z - w = -1 \end{cases}$$

**Exercise 4.**

In Problems 17–24, write the system of equations corresponding to each augmented matrix. Then perform the indicated row operation(s) on the given augmented matrix.

17.  $\left[ \begin{array}{cc|c} 1 & -3 & -2 \\ 2 & -5 & 5 \end{array} \right] \quad R_2 = -2r_1 + r_2$

18.  $\left[ \begin{array}{cc|c} 1 & -3 & -3 \\ 2 & -5 & -4 \end{array} \right] \quad R_2 = -2r_1 + r_2$

19.  $\left[ \begin{array}{ccc|c} 1 & -3 & 4 & 3 \\ 3 & -5 & 6 & 6 \\ -5 & 3 & 4 & 6 \end{array} \right] \quad \begin{array}{l} R_2 = -3r_1 + r_2 \\ R_3 = 5r_1 + r_3 \end{array}$

20.  $\left[ \begin{array}{ccc|c} 1 & -3 & 3 & -5 \\ -4 & -5 & -3 & -5 \\ -3 & -2 & 4 & 6 \end{array} \right] \quad \begin{array}{l} R_2 = 4r_1 + r_2 \\ R_3 = 3r_1 + r_3 \end{array}$

21.  $\left[ \begin{array}{ccc|c} 1 & -3 & 2 & -6 \\ 2 & -5 & 3 & -4 \\ -3 & -6 & 4 & 6 \end{array} \right] \quad \begin{array}{l} R_2 = -2r_1 + r_2 \\ R_3 = 3r_1 + r_3 \end{array}$

22.  $\left[ \begin{array}{ccc|c} 1 & -3 & -4 & -6 \\ 6 & -5 & 6 & -6 \\ -1 & 1 & 4 & 6 \end{array} \right] \quad \begin{array}{l} R_2 = -6r_1 + r_2 \\ R_3 = r_1 + r_3 \end{array}$

23.  $\left[ \begin{array}{ccc|c} 5 & -3 & 1 & -2 \\ 2 & -5 & 6 & -2 \\ -4 & 1 & 4 & 6 \end{array} \right] \quad \begin{array}{l} R_1 = -2r_2 + r_1 \\ R_3 = 2r_2 + r_3 \end{array}$

24.  $\left[ \begin{array}{ccc|c} 4 & -3 & -1 & 2 \\ 3 & -5 & 2 & 6 \\ -3 & -6 & 4 & 6 \end{array} \right] \quad \begin{array}{l} R_1 = -r_2 + r_1 \\ R_3 = r_2 + r_3 \end{array}$

**Exercise 5.**

In Problems 46–60, solve each system of equations using matrices (row operations). If the system has no solution, say that it is inconsistent.

46.  $\begin{cases} 2x - y = -1 \\ x + \frac{1}{2}y = \frac{3}{2} \end{cases}$

47.  $\begin{cases} x - y = 6 \\ 2x - 3z = 16 \\ 2y + z = 4 \end{cases}$

48.  $\begin{cases} 2x + y = -4 \\ -2y + 4z = 0 \\ 3x - 2z = -11 \end{cases}$

49.  $\begin{cases} x - 2y + 3z = 7 \\ 2x + y + z = 4 \\ -3x + 2y - 2z = -10 \end{cases}$

50.  $\begin{cases} 2x + y - 3z = 0 \\ -2x + 2y + z = -7 \\ 3x - 4y - 3z = 7 \end{cases}$

51.  $\begin{cases} 2x - 2y - 2z = 2 \\ 2x + 3y + z = 2 \\ 3x + 2y = 0 \end{cases}$

52.  $\begin{cases} 2x - 3y - z = 0 \\ -x + 2y + z = 5 \\ 3x - 4y - z = 1 \end{cases}$

53.  $\begin{cases} -x + y + z = -1 \\ -x + 2y - 3z = -4 \\ 3x - 2y - 7z = 0 \end{cases}$

54.  $\begin{cases} 2x - 3y - z = 0 \\ 3x + 2y + 2z = 2 \\ x + 5y + 3z = 2 \end{cases}$

55.  $\begin{cases} 2x - 2y + 3z = 6 \\ 4x - 3y + 2z = 0 \\ -2x + 3y - 7z = 1 \end{cases}$

56.  $\begin{cases} 3x - 2y + 2z = 6 \\ 7x - 3y + 2z = -1 \\ 2x - 3y + 4z = 0 \end{cases}$

57.  $\begin{cases} x + y - z = 6 \\ 3x - 2y + z = -5 \\ x + 3y - 2z = 14 \end{cases}$

58.  $\begin{cases} x - y + z = -4 \\ 2x - 3y + 4z = -15 \\ 5x + y - 2z = 12 \end{cases}$

59.  $\begin{cases} x + 2y - z = -3 \\ 2x - 4y + z = -7 \\ -2x + 2y - 3z = 4 \end{cases}$

60.  $\begin{cases} x + 4y - 3z = -8 \\ 3x - y + 3z = 12 \\ x + y + 6z = 1 \end{cases}$

**Exercise 6.**

In problems 7–14, find the value of each determinant

7.  $\begin{vmatrix} 6 & 4 \\ -1 & 3 \end{vmatrix}$

8.  $\begin{vmatrix} 8 & -3 \\ 4 & 2 \end{vmatrix}$

9.  $\begin{vmatrix} -3 & -1 \\ 4 & 2 \end{vmatrix}$

10.  $\begin{vmatrix} -4 & 2 \\ -5 & 3 \end{vmatrix}$

11.  $\begin{vmatrix} 3 & 4 & 2 \\ 1 & -1 & 5 \\ 1 & 2 & -2 \end{vmatrix}$

12.  $\begin{vmatrix} 1 & 3 & -2 \\ 6 & 1 & -5 \\ 8 & 2 & 3 \end{vmatrix}$

13.  $\begin{vmatrix} 4 & -1 & 2 \\ 6 & -1 & 0 \\ 1 & -3 & 4 \end{vmatrix}$

14.  $\begin{vmatrix} 3 & -9 & 4 \\ 1 & 4 & 0 \\ 8 & -3 & 1 \end{vmatrix}$

**Exercise 7.**

In Problems 27–36, solve each system of equations using Cramer's Rule if it is applicable. If Cramer's Rule is not applicable, say so.

$$27. \begin{cases} 2x - 3y = -1 \\ 10x + 10y = 5 \end{cases} \quad 28. \begin{cases} 3x - 2y = 0 \\ 5x + 10y = 4 \end{cases} \quad 29. \begin{cases} 2x + 3y = 6 \\ x - y = \frac{1}{2} \end{cases} \quad 30. \begin{cases} \frac{1}{2}x + y = -2 \\ x - 2y = 8 \end{cases}$$

$$31. \begin{cases} 3x - 5y = 3 \\ 15x + 5y = 21 \end{cases} \quad 32. \begin{cases} 2x - y = -1 \\ x + \frac{1}{2}y = \frac{3}{2} \end{cases} \quad 33. \begin{cases} x + y - z = 6 \\ 3x - 2y + z = -5 \\ x + 3y - 2z = 14 \end{cases}$$

$$34. \begin{cases} x - y + z = -4 \\ 2x - 3y + 4z = -15 \\ 5x + y - 2z = 12 \end{cases} \quad 35. \begin{cases} x + 2y - z = -3 \\ 2x - 4y + z = -7 \\ -2x + 2y - 3z = 4 \end{cases} \quad 36. \begin{cases} x + 4y - 3z = -8 \\ 3x - y + 3z = 12 \\ x + y + 6z = 1 \end{cases}$$

**Exercise 8.**

In Problems 43–50, use properties of determinants to find the value of each determinant if it is known that

$$\begin{vmatrix} x & y & z \\ u & v & w \\ 1 & 2 & 3 \end{vmatrix} = 4$$

$$43. \begin{vmatrix} 1 & 2 & 3 \\ u & v & w \\ x & y & z \end{vmatrix}$$

$$44. \begin{vmatrix} x & y & z \\ u & v & w \\ 2 & 4 & 6 \end{vmatrix}$$

$$45. \begin{vmatrix} x & y & z \\ -3 & -6 & -9 \\ u & v & w \end{vmatrix}$$

$$46. \begin{vmatrix} 1 & 2 & 3 \\ x - u & y - v & z - w \\ u & v & w \end{vmatrix}$$

$$47. \begin{vmatrix} 1 & 2 & 3 \\ x - 3 & y - 6 & z - 9 \\ 2u & 2v & 2w \end{vmatrix}$$

$$48. \begin{vmatrix} x & y & z - x \\ u & v & w - u \\ 1 & 2 & 2 \end{vmatrix}$$

$$49. \begin{vmatrix} 1 & 2 & 3 \\ 2x & 2y & 2z \\ u - 1 & v - 2 & w - 3 \end{vmatrix}$$

$$50. \begin{vmatrix} x + 3 & y + 6 & z + 9 \\ 3u - 1 & 3v - 2 & 3w - 3 \\ 1 & 2 & 3 \end{vmatrix}$$

**Exercise 9.**

In problems 51–56, solve for x

$$51. \begin{vmatrix} x & x \\ 4 & 3 \end{vmatrix} = 5$$

$$52. \begin{vmatrix} x & 1 \\ 3 & x \end{vmatrix} = -2$$

$$53. \begin{vmatrix} x & 1 & 1 \\ 4 & 3 & 2 \\ -1 & 2 & 5 \end{vmatrix} = 2$$

$$54. \begin{vmatrix} 3 & 2 & 4 \\ 1 & x & 5 \\ 0 & 1 & -2 \end{vmatrix} = 0$$

$$55. \begin{vmatrix} x & 2 & 3 \\ 1 & x & 0 \\ 6 & 1 & -2 \end{vmatrix} = 7$$

$$56. \begin{vmatrix} x & 1 & 2 \\ 1 & x & 3 \\ 0 & 1 & 2 \end{vmatrix} = -4x$$

**HOMEWORKS:**

**Exercise 1:** 33, 35, 37

**Exercise 2:** 2

**Exercise 3:** 5, 7, 9

**Exercise 4:** 17, 19, 21

**Exercise 6:** 7, 9, 11, 13

**Exercise 7:** 27, 29

**Exercise 8:** 43, 45, 47

**Exercise 9:** 51, 53, 55